list_int_functions.v
@@ -1,39 +1,77 @@
-Require Import ZArith.
-Require Import stdpp.list.
 Require Import VST.floyd.proofauto.
+Require Import stdpp.list.
+Require Import ZArith.
+Require Import compcert.lib.Coqlib.
+Require Import list_lemmas.
+
 
 (*  Function to split a [large] integer into a list representation 
     of size number of limbs (14 in this case).*)
 
+Definition prime: Z := 2^448 - 2^224 - 1.
+
 Local Open Scope Z. 
 
- Definition int_to_list (N : Z) : list Z := 
-    [    N mod 2^32;             
-        (N/(2^32)) mod 2^32;
-        (N/(2^(32*2))) mod 2^32;
-        (N/(2^(32*3))) mod 2^32;
-        (N/(2^(32*4))) mod 2^32;
-        (N/(2^(32*5))) mod 2^32;
-        (N/(2^(32*6))) mod 2^32;
-        (N/(2^(32*7))) mod 2^32;
-        (N/(2^(32*8))) mod 2^32;
-        (N/(2^(32*9))) mod 2^32;
-        (N/(2^(32*10))) mod 2^32;
-        (N/(2^(32*11))) mod 2^32;
-        (N/(2^(32*12))) mod 2^32;
-        (N/(2^(32*13))) mod 2^32
-    ].
+Fixpoint int_to_list_aux (N : Z) (i : nat) :=
+    match (i) with
+    | 0%nat => nil
+    | S i' => [(N / (2^(32 * (13 - (Z.of_nat i'))))) mod 2^32] ++ int_to_list_aux N i'
+    end.
+
+Definition int_to_list (N : Z) : list Z := 
+    int_to_list_aux N 14.
+
+Definition two_prime_mone_list : list Z :=
+    [4294967293; 4294967295; 4294967295; 4294967295; 4294967295;
+       4294967295; 4294967295; 4294967293; 4294967295; 4294967295;
+       4294967295; 4294967295; 4294967295; 4294967295].
+
+Definition prime_list : list Z := 
+    [2^32-1; 2^32-1; 2^32-1; 2^32-1; 2^32-1;
+     2^32-1; 2^32-1; 2^32-2; 2^32-1; 2^32-1;
+     2^32-1; 2^32-1; 2^32-1; 2^32-1].
+
+Definition f_fun (l : list Z) (i t : Z) : Z:=
+    if (i =? 0) then (Znth i l) + t
+    else  Int.unsigned (Int.shru (Int.repr ((Znth (i-1) l) + t)) (Int.repr 32)). 
+
+Fixpoint list_subtract (l1 l2: list Z) :=
+    match l1, l2 with
+    | [], _ => map (fun a => -1 * a) l2
+    | _, [] => l1
+    | h1::t1, h2::t2 => (h1 - h2)::list_subtract t1 t2
+    end.
+
+Fixpoint list_add_with_temp_aux (l : list Z) (temp : Z) (i : nat) :=
+    match i with 
+    | 0 => 
+    | 
 
 (*  Function (body) to unify the list representation of a large integer 
     so that it is an integer. *)
-Fixpoint list_to_int' (l  : list Z) (n : Z) : Z := 
+Fixpoint list_to_int_aux (l  : list Z) (n : Z) : Z := 
     match l with 
     | nil => 0
-    | h :: t => (h * (Z.pow 2 (32 * (n)))) + (list_to_int' t (n+1))
+    | h :: t => ((h mod 2^32) * (Z.pow 2 (32 * (n)))) + (list_to_int_aux t (n+1))
     end. 
 
 (* Function to write an integer from a list representation. *)
-Definition list_to_int (l : list Z) := list_to_int' l 0.
+Definition list_to_int (l : list Z) := list_to_int_aux l 0.
+
+Compute ((list_to_int [1;1;0;1] - list_to_int [1;0;0;3]) mod 2^(32*4)).
+Compute list_to_int (list_subtract [1;1;0;1] [1;0;0;3]) mod 2^(32*4).
+
+
+
+(* NOTE: int_to_list loses information on numbers greater than prime + 2^(32*7) -- 
+         no problem if doing list_to_int (a-prime) as long as a < 2*prime.*)
+
+Compute (prime - 2^(32*7)).
+
+(* Definition x : Z := prime + 2^(32*7) .
+
+Compute list_to_int (int_to_list x) - x.
+Compute prime. *)
 
 
 (*  Checks if two lists have the same contents, where the contents are  *
@@ -50,3 +88,61 @@ Fixpoint list_Inteq (a b : list Z) : bool :=
                      list_Inteq a b
         end
     end.
+
+(* LEMMAS *)
+
+Lemma  int_to_list_length: 
+forall N : Z, 
+Zlength (int_to_list N) = 14.  
+Proof.
+unfold int_to_list.
+auto. 
+Qed.
+
+Lemma  int_to_list__list_to_int_pres_length:
+forall l : list Z,  
+Zlength (int_to_list (list_to_int l)) = 14.
+Proof.
+    intros.
+    apply int_to_list_length.    
+Qed.
+
+Lemma Znth_int_to_list: 
+forall (N : Z) (i : nat), 
+(Z.of_nat i) < 14 ->
+Znth (Z.of_nat i) (int_to_list N) = (N / (2^(32 * (Z.of_nat i)))) mod 2^32.
+Proof. (* This is a manual proof by induction. *)
+    intros.
+    induction i as [| i _]; try easy.
+    replace (Z.of_nat (S i)) with ((Z.of_nat i)+1) by lia.
+    induction i as [| i _]; try easy.
+    replace (Z.of_nat (S i)) with ((Z.of_nat i)+1) by lia.
+    induction i as [| i _]; try easy;
+    replace (Z.of_nat (S i)) with ((Z.of_nat i)+1) by lia.
+    induction i as [| i _]; try easy;
+    replace (Z.of_nat (S i)) with ((Z.of_nat i)+1) by lia.
+    induction i as [| i _]; try easy;
+    replace (Z.of_nat (S i)) with ((Z.of_nat i)+1) by lia.
+    induction i as [| i _]; try easy;
+    replace (Z.of_nat (S i)) with ((Z.of_nat i)+1) by lia.
+    induction i as [| i _]; try easy;
+    replace (Z.of_nat (S i)) with ((Z.of_nat i)+1) by lia.
+    induction i as [| i _]; try easy;
+    replace (Z.of_nat (S i)) with ((Z.of_nat i)+1) by lia.
+    induction i as [| i _]; try easy;
+    replace (Z.of_nat (S i)) with ((Z.of_nat i)+1) by lia.
+    induction i as [| i _]; try easy;
+    replace (Z.of_nat (S i)) with ((Z.of_nat i)+1) by lia.
+    induction i as [| i _]; try easy;
+    replace (Z.of_nat (S i)) with ((Z.of_nat i)+1) by lia.
+    induction i as [| i _]; try easy;
+    replace (Z.of_nat (S i)) with ((Z.of_nat i)+1) by lia.
+    induction i as [| i _]; try easy;
+    replace (Z.of_nat (S i)) with ((Z.of_nat i)+1) by lia.
+    induction i as [| i _]; try easy;
+    replace (Z.of_nat (S i)) with ((Z.of_nat i)+1) by lia.
+    simpl in H. 
+    replace (Z.of_nat
+    (S (S (S (S (S (S (S (S (S (S (S (S (S (S i))))))))))))))) with 14 in H by lia. 
+    discriminate H. 
+    Qed.
