verif_curve448Add.v
@@ -1,0 +1,362 @@
+Require Import VST.floyd.proofauto.
+Require Import curve448.
+Require Import list_int_functions.
+Require Import stdpp.list.
+Require Import ZArith.
+Require Import compcert.lib.Coqlib.
+Require Import list_lemmas.
+
+Instance CompSpecs : compspecs. Proof. make_compspecs prog. Defined.
+Definition Vprog : varspecs.  mk_varspecs prog. Defined.
+
+Local Open Scope Z.
+
+
+Definition prime: Z := 2^448 - 2^224 - 1.
+
+Definition undef14 :=
+       [Vundef; Vundef; Vundef; Vundef; Vundef; Vundef; Vundef;
+        Vundef; Vundef; Vundef; Vundef; Vundef; Vundef; Vundef].
+
+Lemma L3 (z : Z) : 
+0 <= z < Int64.modulus -> Int64.unsigned (Int64.repr z) = z.
+Proof.
+   intros.
+   rewrite Int64.unsigned_repr_eq.
+   rewrite Z.mod_small; auto.
+Qed.
+
+Lemma  L4' (z : Z): 
+Int.eq (Int.repr z) Int.mone = false -> z mod Int.modulus ≠ Int.modulus - 1.
+Proof.
+   intros.
+   apply int_eq_false_e in H.
+   unfold "≠".
+   intros.
+   replace (Int.modulus - 1) with (Int.modulus - 1 mod Int.modulus) in H0.
+   assert (Int.repr z = Int.repr (Int.modulus - 1)).
+   apply modulo_samerepr.
+   apply H0.
+   replace (Int.repr (Int.modulus - 1)) with (Int.repr (- 1)) in H1.
+   contradiction.
+   rewrite modulo_samerepr with (y:= Int.modulus - 1); reflexivity.
+   apply Zmod_small with (a := Int.modulus - 1) (n:= Int.modulus).
+   easy.
+Qed.
+
+Lemma L4 (z : Z) :
+Int.eq (Int.repr z) Int.mone = false -> z mod Int.modulus < Int.modulus - 1.
+Proof.
+   intros. 
+   apply int_eq_false_e in H.
+   unfold Int.mone in H.
+   apply Znot_ge_lt.
+   unfold not.
+   intros.
+   assert (Int.modulus ≠ 0) by easy.
+   apply Z.mod_bound_or with (a := z) in H1.
+   destruct H1.
+   destruct H1.
+   assert (z mod Int.modulus <= Int.modulus - 1).
+   apply Zlt_succ_le.
+   replace (Z.succ (Int.modulus - 1)) with (Int.modulus) by easy.
+   assumption.
+   assert ( z mod Int.modulus = Int.modulus - 1). 
+   apply Z.ge_le in H0.
+   apply Z.le_antisymm; assumption.
+   replace (Int.modulus - 1) with (- 1 mod Int.modulus) in H4 by easy.
+   apply modulo_samerepr in H4.
+   contradiction.
+   destruct H1.
+   assert (Int.modulus < 0).
+   apply Z.lt_le_trans with (m:= z mod Int.modulus); assumption.
+   discriminate H3. 
+   Qed.
+
+Lemma int64_shru_small (z : Z) : 0 <= z < two_p 32 ->
+   Int64.shru (Int64.repr z) (Int64.repr 32) = Int64.zero.
+Proof.
+   intros.
+   rewrite Int64.shru_div_two_p. 
+   assert (Int64.unsigned (Int64.repr z) / two_p (Int64.unsigned (Int64.repr 32)) = 0).
+   rewrite Zdiv_small; try easy.
+   split.
+   destruct H.
+   rewrite L3; try easy.
+   split; try easy.
+   assert ((two_p 32) < Int64.modulus) by easy.
+   apply Z.lt_trans with (two_p 32); assumption.
+   replace (Int64.unsigned (Int64.repr 32)) with 32 by easy.
+   destruct H.
+   rewrite L3; try easy.
+   split; try easy.
+   assert ((two_p 32) < Int64.modulus) by easy.
+   apply Z.lt_trans with (two_p 32); assumption.
+   rewrite H0. easy.
+Qed. 
+
+Lemma div_eucl_by_hand: forall a b q r: Z,
+0 < b -> 
+0 <= r < b -> 
+a = q * b + r -> 
+Z.div_eucl a b = (q, r).
+Proof.
+    intros.
+    rewrite Zaux.Zdiv_eucl_unique.
+    (* Search (_ -> _ / _ = _). *)
+    rewrite H1 at 1.
+    rewrite Z.div_add_l; try lia.
+    rewrite Z.div_small; try lia.
+    rewrite H1.
+    rewrite Z.add_mod; try lia.
+    rewrite Z.mod_mul; try lia.
+    (* assert ((0 + r mod b) mod b = r). *)
+    replace (0 + r mod b) with (r mod b) by lia.
+    rewrite Z.mod_mod; try lia.
+    rewrite Z.mod_small; try lia.
+    replace (q + 0) with (q) by lia.
+    reflexivity.
+Qed.
+
+Lemma  div_bound_double: forall n z : Z,
+0 < n -> 
+n <= z < 2 * n -> 
+z / n = 1.
+Proof.
+    intros.
+    unfold "/".
+    assert (Z.div_eucl z (n) = (1, z-n)). 
+    assert (z = n + (z - n)) by lia.
+    rewrite div_eucl_by_hand with (q:= 1) (r:= z - n); try lia.
+    reflexivity.
+    rewrite H1.
+    reflexivity.
+Qed.
+
+Lemma int64_shru_big (z : Z) : two_p 32 <= z < two_p 33 ->
+   Int64.shru (Int64.repr z) (Int64.repr 32) = Int64.one.
+Proof.
+    intros.
+    rewrite Int64.shru_div_two_p.
+    replace (Int64.unsigned (Int64.repr 32)) with 32 by easy. 
+    rewrite L3.
+    assert (z / two_p 32 = 1).
+    apply div_bound_double; try easy.
+    rewrite H0; easy.
+    destruct H.
+    split.
+    assert (0 <= two_p 32) by easy.
+    lia.  
+    assert (two_p 33 < Int64.modulus) by easy.
+    lia.
+Qed. 
+
+(* %%%%%%%%%%%%%%%%%%%%%%%%% *)
+Definition curve448Add_spec : ident * funspec :=
+DECLARE _curve448Add
+WITH    r : val,
+        shr : share,
+        a : val,
+        contents_a : list Z,
+        b : val,
+        contents_b : list Z,
+        gv : globals
+PRE [ tptr tuint, tptr tuint, tptr tuint ]
+    PROP   (writable_share shr;
+            Zlength contents_a = 14;
+            Zlength contents_b = 14;
+            0 <= (list_to_int contents_a) < prime;
+            0 <= (list_to_int contents_b) < prime;
+            forall x : Z, In x contents_a → 0 <= x < 2 ^ 32 /\ x mod Int.modulus < 2^32;
+            forall x : Z, In x contents_b → 0 <= x < 2 ^ 32 /\ x mod Int.modulus < 2^32)
+    PARAMS (r ; a ; b) GLOBALS (gv)
+    SEP    (data_at_ shr (tarray tuint 14) r;
+            data_at Tsh (tarray tuint 14) (map Vint (map Int.repr contents_a)) a;
+            data_at Tsh (tarray tuint 14) (map Vint (map Int.repr contents_b)) b)
+POST [ tvoid ]
+    PROP   ()
+    RETURN ()
+    SEP    (data_at shr (tarray tuint 14) (* r contains the representation of A + B mod p *)
+   (*cont*)(map Vint (map Int.repr (int_to_list (((list_to_int contents_a) + (list_to_int contents_b)) mod prime)))) r ;
+            data_at Tsh (tarray tuint 14) (map Vint (map Int.repr contents_a)) a ;
+            data_at Tsh (tarray tuint 14) (map Vint (map Int.repr contents_b)) b).
+
+Definition carrying (i : Z) (a b : list Z) : bool:=
+        if (i =? 0) then false
+        else ((Znth i a) + (Znth i b)) >=? 2^32.
+
+Definition curve448Add_INV  (a : val)  (contents_a : list Z)
+                            (b : val)  (contents_b : list Z)
+                            (r : val) (shr : share) (gv : globals) :=
+    (EX i : Z, EX t : int64,
+    (PROP   (Zlength contents_a = 14; Zlength contents_b = 14;
+             t = Int64.zero \/ t = Int64.one)
+    LOCAL   (temp _a a; temp _b b; temp _r r;
+            temp _temp (Vlong t);
+            gvars gv)
+    SEP     (  data_at Tsh (tarray tuint 14) (map Vint (map Int.repr contents_a)) a;
+               data_at Tsh (tarray tuint 14) (map Vint (map Int.repr contents_b)) b;
+               data_at shr (tarray tuint 14)
+               ((sublist.sublist 0 i (map Vint (map Int.repr
+                     (int_to_list ((list_to_int contents_a + list_to_int contents_b) mod prime)))))
+               ++ sublist.sublist i 14 undef14) r
+            )))%assert.
+
+Definition Gprog : funspecs := ltac:(with_library prog [ curve448Add_spec ]).
+
+Lemma body_curve448Red : semax_body Vprog Gprog f_curve448Add curve448Add_spec.
+Proof.
+    start_function.
+    forward.
+    forward_for_simple_bound 14
+    (curve448Add_INV a contents_a b contents_b r shr gv).
+    Exists (Int64.repr 0). 
+    entailer!.
+    easy.
+    repeat forward.
+    entailer!.
+    Exists ((Int64.shru
+    (Int64.add
+       (Int64.add t
+          (Int64.repr
+             (Int.unsigned
+                (Int.repr (Znth i contents_a)))))
+       (Int64.repr
+          (Int.unsigned (Int.repr (Znth i contents_b)))))
+    (Int64.repr (Int.unsigned (Int.repr 32))))).
+    entailer!.
+    destruct H6; rewrite H6. 
+    rewrite Int64.add_zero_l.
+    autorewrite with norm.
+    assert (sum: ((((Int.unsigned (Int.repr (Znth i contents_a)) 
+                    + Int.unsigned (Int.repr (Znth i contents_b)))) < 2^32) 
+            \/ 2^32 <= ((Int.unsigned (Int.repr (Znth i contents_a)) 
+                    + Int.unsigned (Int.repr (Znth i contents_b)))))) by lia.
+    destruct sum as [sum_lt | sum_ge].
+    left.
+    rewrite int64_shru_small; try easy.
+    split.
+    apply Z.add_nonneg_nonneg; apply Int64.int_unsigned_range.
+    replace (two_p 32) with (2^32) by easy; assumption.
+    right.
+    apply int64_shru_big.
+    split.
+    replace (two_p 32) with (2^32) by easy; assumption.
+    assert (Int.unsigned (Int.repr (Znth i contents_a)) < 2^32).
+    rewrite Int.unsigned_repr_eq.
+    apply H3.
+    apply Znth_In; lia.
+    assert (Int.unsigned (Int.repr (Znth i contents_b)) < 2^32).
+    rewrite Int.unsigned_repr_eq.
+    apply H4.
+    apply Znth_In; lia.
+    replace (two_p 33) with (2^32 + 2^32) by easy.
+    apply Z.add_lt_mono; assumption. 
+    (* Case where t = 1. *)
+    rewrite Int64.add_assoc.
+    autorewrite with norm.
+    unfold Int64.add.
+    rewrite Int64.unsigned_one.
+    autorewrite with norm. 
+    assert (sum: ((((1 + Int.unsigned (Int.repr (Znth i contents_a)) 
+                    + Int.unsigned (Int.repr (Znth i contents_b)))) < 2^32 ) 
+            \/ 2^32 <= ((1 + Int.unsigned (Int.repr (Znth i contents_a)) 
+                    + Int.unsigned (Int.repr (Znth i contents_b)))))) by lia.
+    destruct sum as [sum_lt | sum_ge].
+    left.
+    rewrite int64_shru_small; try easy.
+    split.
+    apply Z.add_nonneg_nonneg; try easy.
+    apply Z.add_nonneg_nonneg; apply Int64.int_unsigned_range.
+    replace (two_p 32) with (2^32) by easy; lia.
+    right.
+    rewrite int64_shru_big; try easy.
+    split.
+    replace (two_p 32) with (2^32) by easy; lia.
+    assert (Int.unsigned (Int.repr (Znth i contents_a)) < 2^32).
+    rewrite Int.unsigned_repr_eq.
+    apply H3.
+    apply Znth_In; lia.
+    assert (Int.unsigned (Int.repr (Znth i contents_b)) < 2^32).
+    rewrite Int.unsigned_repr_eq.
+    apply H4.
+    apply Znth_In; lia.
+    replace (two_p 33) with (2^32 + 2^32) by easy.
+    rewrite Z.add_assoc.
+    apply Z.add_le_lt_mono; lia.
+    assert (data_at_r : (upd_Znth i
+     (sublist.sublist 0 i 
+     (map Vint (map Int.repr (int_to_list ((list_to_int contents_a + list_to_int contents_b) mod prime)))) ++
+      sublist.sublist i 14 undef14)
+     (Vint
+        (Int.repr
+           (Int64.unsigned
+              (Int64.and
+                 (Int64.add (Int64.add t (Int64.repr (Int.unsigned (Int.repr (Znth i contents_a)))))
+                    (Int64.repr (Int.unsigned (Int.repr (Znth i contents_b)))))
+                 (Int64.repr (Int.unsigned (Int.repr (-1))))))))) =
+      (sublist.sublist 0 (i + 1)
+         (map Vint
+            (map Int.repr (int_to_list ((list_to_int contents_a + list_to_int contents_b) mod prime)))) ++
+       sublist.sublist (i + 1) 14 undef14) ).
+
+
+    rewrite <- !(sublist_rejoin 0 i (i+1)); try easy.
+    rewrite <- app_assoc.   
+    rewrite upd_list_app_upper.
+    rewrite Zlength_sublist; try easy.
+    autorewrite with sublist.  
+    rewrite sublist_update_0th_gen; try easy; try lia.
+    rewrite sublist_len_1.
+    repeat f_equal.
+
+    rewrite Znth_map_Vint_map_Int_repr.
+    replace (i) with (Z.of_nat (Z.to_nat i)) by lia.
+    rewrite Znth_int_to_list.
+    f_equal.
+    replace (Z.of_nat (Z.to_nat i)) with i by lia. 
+    autorewrite with sublist in *|-.
+    About Vlong.
+    assert ((Znth i contents_a = -1) \/ (Znth i contents_a <> -1)).
+    lia.
+    destruct H10; try rewrite H10.
+    replace ((Int64.add Int64.one (Int64.repr (Int.unsigned (Int.repr (-1)))))) 
+    with (Int64.repr(2^32)) by easy.
+    replace ((Int64.and (Int64.repr (2 ^ 32))
+    (Int64.repr (Int.unsigned (Int.repr (-1)))))) with (Int64.zero) by easy.
+    replace (Int.repr (Int64.unsigned Int64.zero)) with (Int.repr 0) by easy.
+    simpl.
+admit.
+
+rewrite data_at_r; easy.
+
+Intros t.
+
+(* Need Red. *)
+
+
+
+
+
+    
+    
+
+
+(* void curve448Add(uint32_t *r, const uint32_t *a, const uint32_t *b)
+{
+   uint_t i;
+   uint64_t temp;
+
+   //Compute R = A + B
+   temp = 0;
+   for(i = 0; i < 14; i++)
+   {
+      temp += a[i];
+      temp += b[i];
+      r[i] = temp & 0xFFFFFFFF;
+      temp >>= 32;
+   }
+
+   //Perform modular reduction
+   curve448Red(r, r, (uint32_t) temp);
+} *)
