verif_curve448AddInt.v
@@ -1,0 +1,597 @@
+Require Import VST.floyd.proofauto.
+Require Import curve448.
+Require Import list_int_functions.
+Require Import stdpp.list.
+Require Import ZArith.
+Require Import compcert.lib.Coqlib.
+Require Import list_lemmas.
+
+Instance CompSpecs : compspecs. Proof. make_compspecs prog. Defined.
+Definition Vprog : varspecs.  mk_varspecs prog. Defined.
+
+Local Open Scope Z.
+
+Definition prime: Z := 2^448 - 2^224 - 1.
+
+Definition undef14 :=
+       [Vundef; Vundef; Vundef; Vundef; Vundef; Vundef; Vundef;
+        Vundef; Vundef; Vundef; Vundef; Vundef; Vundef; Vundef].
+
+(* Functions to compute added lists. *)
+Definition is_big (n : Z) (a : list Z) (b : Z) := 
+   if (n =? 0) 
+      then Znth n a + b >=? Int.modulus
+      else Int.eq (Int.repr (Znth n a)) Int.mone.
+
+Fixpoint allprev_big_aux (n : nat) (a : list Z) (b : Z) : bool :=
+   match n with 
+   | O   => true
+   | S n' => is_big (Z.of_nat n') a b
+            && allprev_big_aux n' a b
+   end.
+   
+Definition allprev_big (i b : Z) (a : list Z) :=
+   allprev_big_aux (Z.to_nat i) a b.
+
+Definition allprev_big_compute (i b : Z) (a : list Z) :=
+   if (i =? 0) then Vlong (Int64.repr b)
+   else if (allprev_big i b a) 
+                        then Vlong Int64.one
+                        else Vlong Int64.zero.
+
+Fixpoint added_list_aux (n : nat) (b : Z) (a : list Z):=
+   match n with 
+   | O    => [(Znth (Z.of_nat n) a) + b]
+   | S n' => added_list_aux n' b a ++
+             [(Znth (Z.of_nat (S n')) a) 
+             + (if (allprev_big (Z.of_nat (S n')) b a) then 1 else 0) mod Int.modulus]
+   end.
+
+Definition added_list (a : list Z) (b : Z):=
+   added_list_aux 13 b a.
+(* %%%%%%%%%%%%%%%%%%%%%%%%%%%%%%%%%%%%%%%%%%%%%%%%%%%%%%%%%%%%%%%%% *)
+(* %%%%%%%%%%%%% Lemmas about added_lists %%%%%%%%%%%%% *)
+Lemma zlength_added_list: 
+forall a: list Z, forall b : Z,
+Zlength (added_list a b) = 14.
+Proof.
+   intros.
+   unfold added_list.
+   unfold added_list_aux.
+   list_solve.
+Qed.
+
+Lemma znth_added_list:
+forall i:nat, forall b: Z, forall a : list Z, 
+0 < (Z.of_nat i) < Zlength (added_list a b) -> 
+Znth (Z.of_nat i) (added_list a b) = 
+         Znth (Z.of_nat i) a +
+         (if allprev_big (Z.of_nat i) b a then 1 else 0) mod Int.modulus.
+Proof. (* By manual induction for now. *)
+   intros.
+   destruct i.
+   destruct H; discriminate H. 
+   replace (Z.of_nat (S i)) with ((Z.of_nat i)+1) in * by lia. 
+   destruct i. unfold added_list; unfold added_list_aux; list_solve;
+   replace (Z.of_nat (S i)) with ((Z.of_nat i)+1) in * by lia.  
+   destruct i. unfold added_list; unfold added_list_aux; list_solve;
+   replace (Z.of_nat (S i)) with ((Z.of_nat i)+1) in * by lia. 
+   destruct i. unfold added_list; unfold added_list_aux; list_solve;
+   replace (Z.of_nat (S i)) with ((Z.of_nat i)+1) in * by lia. 
+   destruct i. unfold added_list; unfold added_list_aux; list_solve;
+   replace (Z.of_nat (S i)) with ((Z.of_nat i)+1) in * by lia.
+   destruct i. unfold added_list; unfold added_list_aux; list_solve;
+   replace (Z.of_nat (S i)) with ((Z.of_nat i)+1) in * by lia.
+   destruct i. unfold added_list; unfold added_list_aux; list_solve;
+   replace (Z.of_nat (S i)) with ((Z.of_nat i)+1) in * by lia.
+   destruct i. unfold added_list; unfold added_list_aux; list_solve;
+   replace (Z.of_nat (S i)) with ((Z.of_nat i)+1) in * by lia.
+   destruct i. unfold added_list; unfold added_list_aux; list_solve;
+   replace (Z.of_nat (S i)) with ((Z.of_nat i)+1) in * by lia.
+   destruct i. unfold added_list; unfold added_list_aux; list_solve;
+   replace (Z.of_nat (S i)) with ((Z.of_nat i)+1) in * by lia.
+   destruct i. unfold added_list; unfold added_list_aux; list_solve;
+   replace (Z.of_nat (S i)) with ((Z.of_nat i)+1) in * by lia.
+   destruct i. unfold added_list; unfold added_list_aux; list_solve;
+   replace (Z.of_nat (S i)) with ((Z.of_nat i)+1) in * by lia.
+   destruct i. unfold added_list; unfold added_list_aux; list_solve;
+   replace (Z.of_nat (S i)) with ((Z.of_nat i)+1) in * by lia.
+   destruct i. unfold added_list; unfold added_list_aux; list_solve;
+   replace (Z.of_nat (S i)) with ((Z.of_nat i)+1) in * by lia.
+   rewrite zlength_added_list in H.
+   assert (Z.of_nat (S (S (S (S (S (S (S (S (S (S (S (S (S i))))))))))))) + 1 >= 14) by lia.
+   destruct H.
+   lia.
+Qed.
+   
+Lemma allprev_big_unfoldable :
+   forall (i b : Z) (a : list Z),
+   0 <= i -> 
+   0 <= b < 2^32-1 ->
+   allprev_big (i + 1) b a = 
+   is_big i a b && allprev_big i b a.
+Proof.
+   intros.
+   unfold allprev_big.
+   replace (i + 1) with (Z.succ i) by easy.
+   rewrite Z2Nat.inj_succ by apply H.
+   assert (i = Z.of_nat (Z.to_nat i)) by
+      ((rewrite Z2Nat.id; auto)).
+   rewrite H1 at 2.
+   induction (Z.to_nat i); auto.
+Qed.
+(* %%%%%%%%%%%%% General Lemmas %%%%%%%%%%%%% *) 
+Lemma L3 (z : Z) : 
+0 <= z < Int64.modulus -> Int64.unsigned (Int64.repr z) = z.
+Proof.
+   intros.
+   rewrite Int64.unsigned_repr_eq.
+   rewrite Z.mod_small; auto.
+Qed.
+
+Lemma  L4' (z : Z): 
+Int.eq (Int.repr z) Int.mone = false -> z mod Int.modulus ≠ Int.modulus - 1.
+Proof.
+   intros.
+   apply int_eq_false_e in H.
+   unfold "≠".
+   intros.
+   replace (Int.modulus - 1) with (Int.modulus - 1 mod Int.modulus) in H0.
+   assert (Int.repr z = Int.repr (Int.modulus - 1)).
+   apply modulo_samerepr.
+   apply H0.
+   replace (Int.repr (Int.modulus - 1)) with (Int.repr (- 1)) in H1.
+   contradiction.
+   rewrite modulo_samerepr with (y:= Int.modulus - 1); reflexivity.
+   apply Zmod_small with (a := Int.modulus - 1) (n:= Int.modulus).
+   easy.
+Qed.
+
+Lemma L4 (z : Z) :
+Int.eq (Int.repr z) Int.mone = false -> z mod Int.modulus < Int.modulus - 1.
+Proof.
+   intros. 
+   apply int_eq_false_e in H.
+   unfold Int.mone in H.
+   apply Znot_ge_lt.
+   unfold not.
+   intros.
+   assert (Int.modulus ≠ 0) by easy.
+   apply Z.mod_bound_or with (a := z) in H1.
+   destruct H1.
+   destruct H1.
+   assert (z mod Int.modulus <= Int.modulus - 1).
+   apply Zlt_succ_le.
+   replace (Z.succ (Int.modulus - 1)) with (Int.modulus) by easy.
+   assumption.
+   assert ( z mod Int.modulus = Int.modulus - 1). 
+   apply Z.ge_le in H0.
+   apply Z.le_antisymm; assumption.
+   replace (Int.modulus - 1) with (- 1 mod Int.modulus) in H4 by easy.
+   apply modulo_samerepr in H4.
+   contradiction.
+   destruct H1.
+   assert (Int.modulus < 0).
+   apply Z.lt_le_trans with (m:= z mod Int.modulus); assumption.
+   discriminate H3. 
+   Qed.
+
+Lemma int64_shru_small (z : Z) : 0 <= z < two_p 32 ->
+   Int64.shru (Int64.repr z) (Int64.repr 32) = Int64.zero.
+Proof.
+   intros.
+   rewrite Int64.shru_div_two_p. 
+   assert (Int64.unsigned (Int64.repr z) / two_p (Int64.unsigned (Int64.repr 32)) = 0).
+   rewrite Zdiv_small; try easy.
+   split.
+   destruct H.
+   rewrite L3; try easy.
+   split; try easy.
+   assert ((two_p 32) < Int64.modulus) by easy.
+   apply Z.lt_trans with (two_p 32); assumption.
+   replace (Int64.unsigned (Int64.repr 32)) with 32 by easy.
+   destruct H.
+   rewrite L3; try easy.
+   split; try easy.
+   assert ((two_p 32) < Int64.modulus) by easy.
+   apply Z.lt_trans with (two_p 32); assumption.
+   rewrite H0. easy.
+Qed. 
+
+Lemma div_eucl_by_hand: forall a b q r: Z,
+0 < b -> 
+0 <= r < b -> 
+a = q * b + r -> 
+Z.div_eucl a b = (q, r).
+Proof.
+    intros.
+    rewrite Zaux.Zdiv_eucl_unique.
+    rewrite H1 at 1.
+    rewrite Z.div_add_l; try lia.
+    rewrite Z.div_small; try lia.
+    rewrite H1.
+    rewrite Z.add_mod; try lia.
+    rewrite Z.mod_mul; try lia.
+    (* assert ((0 + r mod b) mod b = r). *)
+    replace (0 + r mod b) with (r mod b) by lia.
+    rewrite Z.mod_mod; try lia.
+    rewrite Z.mod_small; try lia.
+    replace (q + 0) with (q) by lia.
+    reflexivity.
+Qed.
+
+Lemma  div_bound_double: forall n z : Z,
+0 < n -> 
+n <= z < 2 * n -> 
+z / n = 1.
+Proof.
+    intros.
+    unfold "/".
+    assert (Z.div_eucl z (n) = (1, z-n)). 
+    assert (z = n + (z - n)) by lia.
+    rewrite div_eucl_by_hand with (q:= 1) (r:= z - n); try lia.
+    reflexivity.
+    rewrite H1.
+    reflexivity.
+Qed.
+
+Lemma int64_shru_big (z : Z) : two_p 32 <= z < two_p 33 ->
+   Int64.shru (Int64.repr z) (Int64.repr 32) = Int64.one.
+Proof.
+    intros.
+    rewrite Int64.shru_div_two_p.
+    replace (Int64.unsigned (Int64.repr 32)) with 32 by easy. 
+    rewrite L3.
+    assert (z / two_p 32 = 1).
+    apply div_bound_double; try easy.
+    rewrite H0; easy.
+    destruct H.
+    split.
+    assert (0 <= two_p 32) by easy.
+    lia.  
+    assert (two_p 33 < Int64.modulus) by easy.
+    lia.
+Qed. 
+
+Lemma repr_eq_32_64: forall n:Z, 
+   Int.repr (Int64.unsigned (Int64.repr (n))) = Int.repr (Int.unsigned (Int.repr (n))).
+Proof.
+   intros.
+   rewrite Int64.unsigned_repr_eq.
+   rewrite Int.unsigned_repr_eq.
+   rewrite modulo_samerepr with (y:= n mod Int.modulus); try easy.
+   replace (Int64.modulus) with (Int.modulus * Int.modulus) by easy.
+   rewrite Zaux.Zmod_mod_mult; try easy.
+   symmetry; apply Zmod_mod.    
+Qed.   
+
+Lemma L6: forall x : Z,
+0 <= x < Int.modulus -> Int64.unsigned (Int64.repr x) = Int.unsigned (Int.repr x).
+Proof.
+   intros.
+   assert (x = Int.unsigned(Int.repr x)).
+   rewrite Int.unsigned_repr_eq.
+   rewrite Z.mod_small; try lia.
+   rewrite H0.
+   rewrite Int64.int_unsigned_repr.
+   rewrite H0 at 1.
+   easy.
+Qed.
+
+Lemma L7: 
+forall x y,
+0 <= x < Int.modulus -> 0 < y <= 32 -> 
+(Z.land x (Z.ones y)) mod Int.modulus = Z.land x (Z.ones y).
+Proof.
+   intros.
+   rewrite Z.mod_small; try easy.
+   split.
+   apply Z.land_nonneg.
+   lia. 
+   rewrite Z.land_ones; try lia.
+   replace (Int.modulus) with (2^32) by easy.
+   assert (A1 : x mod 2 ^ y < 2^y).
+   apply Z.mod_pos_bound; lia.
+   assert (A2 : 2 ^ y <= 2 ^ 32).
+   destruct H0.
+   apply Z.pow_le_mono_r; try lia.
+   apply Z.lt_le_trans with (m:= 2^y); try lia.
+Qed.
+
+Lemma lt_max_unsigned_iff_le_mod: forall x : Z,
+x <= Int.max_unsigned <-> x < Int.modulus.
+Proof.
+   replace Int.max_unsigned with (2^32-1) by easy.
+   replace Int.modulus with (2^32) by easy.
+   lia.
+Qed.
+
+(* %%%%%%%%%%%%%%%%%%%%%%%%%%%%%%%%%%%%%%%%%%%%%%%%%%%%%%%%%%%%%%%%%%%%%%%%%%% *)
+Definition curve448AddInt_spec : ident * funspec :=
+DECLARE _curve448AddInt
+WITH    r : val,
+        shr : share,
+        a : val,
+        contents_a : list Z,
+        b : Z,
+        gv : globals
+PRE [ tptr tuint, tptr tuint, tuint]
+    PROP   (writable_share shr;
+            Zlength contents_a = 14;
+            0 <= (list_to_int contents_a) < prime; 0 <= b < 2^32 - 1;
+            forall x : Z, In x contents_a → 0 <= x < 2 ^ 32 /\ x mod Int.modulus < 2^32)
+    PARAMS (r ; a ; Vint (Int.repr b)) GLOBALS (gv)
+    SEP    (data_at_ shr (tarray tuint 14) r;
+            data_at Tsh (tarray tuint 14) (map Vint (map Int.repr contents_a)) a)
+POST [ tvoid ]
+    PROP   ()
+    RETURN ()
+    SEP    (data_at shr (tarray tuint 14) (* r contains the representation of A + B mod p *)
+   (*cont*)(map Vint (map Int.repr (int_to_list (((list_to_int contents_a) + (b)) mod prime)))) r ;
+            data_at Tsh (tarray tuint 14) (map Vint (map Int.repr contents_a)) a ).
+
+Definition curve448AddInt_INV  (a : val)  (contents_a : list Z)
+                            (b : Z)
+                            (r : val) (shr : share) (gv : globals) :=
+    (EX i : Z,
+    (PROP   (Zlength contents_a = 14)
+    (* ;t = (Int64.repr b) \/ t = Int64.one \/ t = Int64.zero) *)
+    LOCAL   (temp _a a; temp _r r;
+            temp _temp (allprev_big_compute i b contents_a);
+            gvars gv)
+    SEP     (
+            data_at Tsh (tarray tuint 14) (map Vint (map Int.repr contents_a)) a;
+            data_at shr (tarray tuint 14)
+            (
+               (sublist.sublist 0 i (map Vint (map Int.repr (added_list contents_a b))))
+               ++ (sublist.sublist i 14 undef14)
+            )
+            r)
+    ))%assert.
+
+Definition Gprog : funspecs := ltac:(with_library prog [ curve448AddInt_spec ])(*add red here*).
+
+Lemma body_curve448AddInt : semax_body Vprog Gprog f_curve448AddInt curve448AddInt_spec.
+Proof.
+   start_function.
+   forward.
+   forward_for_simple_bound 14
+   (curve448AddInt_INV a contents_a b r shr gv).
+   entailer!.
+   easy.
+   repeat forward.
+   entailer!.
+   assert (a_i_bound : 0 <= Znth i contents_a < 2^32).
+      apply H2; apply Znth_In; lia.
+   unfold allprev_big_compute.
+   rewrite allprev_big_unfoldable by lia.
+   destruct (allprev_big i b contents_a) eqn : E_prev;
+   destruct (i+1 =? 0) eqn : E_succ;
+   destruct (i =? 0) eqn : E_i;
+   simpl; try lia; try rewrite andb_true_r; try rewrite andb_false_r;
+   try rewrite Z.eqb_eq in *; try rewrite Z.eqb_neq in *;
+   try rewrite E_i in *.
+   unfold is_big; simpl.
+
+   unfold Int64.add.
+   assert (b_bound : 0 <= b < Int.modulus);
+   replace Int.modulus with (2^32) by easy; try lia.
+   repeat rewrite L6; try easy; try apply Int.unsigned_range.
+   repeat rewrite Int.unsigned_repr; try easy; 
+   try (replace Int.max_unsigned with (2^32-1) by easy); try lia.
+   destruct (Znth 0 contents_a + b >=? 2^32) eqn : a_geq_b; simpl.
+   rewrite Z.geb_le in a_geq_b.
+   rewrite int64_shru_big; auto.
+   split; rewrite two_p_equiv; try lia.
+   rewrite int64_shru_small; auto.
+   split; try rewrite two_p_equiv; try lia.
+
+   unfold is_big. 
+   assert (i_not0: i=?0 = false) by lia; rewrite i_not0.
+   unfold Int64.add. 
+   destruct (Int.eq (Int.repr (Znth i contents_a)) Int.mone) eqn: aimone.
+   apply Int.same_if_eq in aimone.
+   unfold Int.mone in aimone.
+   rewrite aimone.
+   replace (Int.unsigned (Int.repr (-1))) with (2^32 -1) by easy.
+   repeat rewrite Int64.unsigned_repr; try easy.
+   
+   apply L4 in aimone.
+   rewrite int64_shru_small; auto.
+   split; try lia.
+      apply Z.add_nonneg_nonneg;
+      apply Int64.unsigned_range.
+      rewrite two_p_equiv.
+      unfold Int64.one.
+      repeat rewrite Int64.unsigned_repr; try easy.
+      rewrite Int.unsigned_repr_eq.
+      replace (Int.modulus) with (2^32) in aimone at 2 by easy.
+      lia.
+      split; try apply Int.unsigned_range.
+      rewrite Int.unsigned_repr_eq.
+      assert (Int.modulus - 1 < Int64.max_unsigned) by easy;
+      lia.
+
+   discriminate E_prev.
+
+   rewrite Int64.add_zero_l.
+      rewrite int64_shru_small; auto.
+      rewrite two_p_equiv. 
+      rewrite Int.unsigned_repr; auto.
+      replace (Int.max_unsigned) with (2^32-1); try easy; try lia.
+
+   (* Prove that if loop inv holds after i then it holds after doing the 
+      i+1 iteration. *)
+   assert (a_i_bound : 0 <= Znth i contents_a < 2^32).
+      apply H2; apply Znth_In; lia.
+   assert (b_bound : 0 <= b < Int.modulus).
+      replace Int.modulus with (2^32) by easy; try lia.
+   assert (b_64bound : 0 <= b <= Int64.max_unsigned). 
+      split; try easy;
+      assert (2^32-1 < Int64.max_unsigned) by easy; lia.
+   assert (data_at_r : (upd_Znth i
+   (sublist.sublist 0 i (map Vint (map Int.repr (added_list contents_a b))) ++
+    sublist.sublist i 14 undef14)
+   (force_val
+      (sem_cast_l2i I32 Unsigned
+         (force_val
+            (sem_and tulong tuint
+               (force_val
+                  (both_long (λ n1 n2 : int64, Some (Vlong (Int64.add n1 n2)))
+                     sem_cast_pointer (sem_cast_i2l Unsigned)
+                     (allprev_big_compute i b contents_a)
+                     (Vint (Int.repr (Znth i contents_a))))) (Vint (Int.repr (-1))))))))
+   =
+   (sublist.sublist 0 (i + 1) (map Vint (map Int.repr (added_list contents_a b))) ++
+       sublist.sublist (i + 1) 14 undef14)).
+
+   rewrite <- !(sublist_rejoin 0 i (i+1)); try easy.
+   rewrite <- app_assoc.   
+   rewrite upd_list_app_upper.
+   assert (len_sublist : Zlength (sublist.sublist 0 i (map Vint (map Int.repr (added_list contents_a b)))) = i).
+   rewrite calc_Zlength_sublist with (len := 14); try easy; try lia.
+   rewrite len_sublist; autorewrite with sublist.
+   rewrite sublist_update_0th_gen; try easy; try lia.
+   rewrite sublist_len_1.
+   repeat f_equal.
+   autorewrite with sublist.
+   unfold allprev_big_compute.
+
+   destruct (i=?0) eqn: i_0.
+   rewrite Z.eqb_eq in i_0; rewrite i_0 in *.
+   unfold added_list.
+   unfold added_list_aux.
+   autorewrite with sublist.
+   simpl.
+   f_equal.
+   unfold Int64.and.
+   replace (Int64.unsigned (Int64.repr (Int.unsigned (Int.repr (-1))))) 
+      with (Z.ones 32) by easy.
+   rewrite Z.land_ones by easy.
+   rewrite L6.
+   rewrite Int.unsigned_repr.
+   unfold Int64.add.
+   rewrite Int64.int_unsigned_repr.
+   rewrite Int.unsigned_repr.
+   rewrite Int64.unsigned_repr.
+   rewrite Int64.unsigned_repr.
+   apply modulo_samerepr.
+   replace (Z.of_nat 0) with 0 by easy.
+   replace (2^32) with Int.modulus by easy.
+   rewrite Z.mod_mod by easy.
+   rewrite Z.add_comm; lia.
+   lia.
+   rewrite Int64.unsigned_repr by lia.
+   split.
+   apply Z.add_nonneg_nonneg; try easy.
+   assert (Int.modulus + 2^32 < Int64.max_unsigned) by easy; lia.
+   replace Int.max_unsigned with (2^32-1) by easy. lia.
+   split.
+   apply Z.mod_bound_pos; try easy.
+   apply Int64.unsigned_range.
+   apply lt_max_unsigned_iff_le_mod.
+   apply Z.mod_bound_pos; try easy; try apply Int64.unsigned_range.
+   split.
+   apply Z.mod_bound_pos; try easy.
+   apply Int64.unsigned_range.
+   apply Z.mod_bound_pos; try easy; try apply Int64.unsigned_range.
+
+   rewrite Z.eqb_neq in i_0.
+   
+   replace (i) with (Z.of_nat (Z.to_nat i)) at 3 by lia.
+   rewrite znth_added_list.
+   replace (Z.of_nat (Z.to_nat i)) with i by lia.
+   destruct (allprev_big i b contents_a) eqn: E_prev; simpl.
+   unfold Int64.and.
+   replace (Int64.unsigned (Int64.repr (Int.unsigned (Int.repr (-1))))) 
+      with (Z.ones 32) by easy.
+   rewrite Z.land_ones by easy.
+   rewrite L6.
+   rewrite Int.unsigned_repr_eq.
+   unfold Int64.add.
+   rewrite Int64.int_unsigned_repr.
+   rewrite Int.unsigned_repr.
+   rewrite Int64.unsigned_repr.
+   unfold Int64.one.
+   rewrite Int64.unsigned_repr by easy.
+   f_equal.
+   apply modulo_samerepr.
+   rewrite Z.mod_mod by easy.
+   replace (2^32) with (Int.modulus) by easy.
+   rewrite Z.mod_mod by easy.
+   rewrite Z.add_comm.
+   easy.
+      replace (Int64.unsigned Int64.one) with (1) by easy.
+      replace (Int64.max_unsigned) with (2^64-1) by easy; lia.
+      rewrite lt_max_unsigned_iff_le_mod. easy.
+      apply Z.mod_bound_pos; try easy; try apply Int64.unsigned_range.
+
+   unfold Int64.and.
+   replace (Int64.unsigned (Int64.repr (Int.unsigned (Int.repr (-1))))) 
+      with (Z.ones 32) by easy.
+   rewrite Z.land_ones by easy.
+   rewrite L6.
+   rewrite Int.unsigned_repr_eq.
+   rewrite Int64.add_zero_l.
+   rewrite Int64.int_unsigned_repr.
+   rewrite Int.unsigned_repr.
+   f_equal.
+   autorewrite with norm.
+   rewrite Z.mod_mod by easy.
+   rewrite modulo_samerepr with (y:=Znth i contents_a); auto.
+   rewrite Z.mod_mod by easy.
+   lia.
+      rewrite lt_max_unsigned_iff_le_mod; easy.
+      apply Z.mod_bound_pos; try easy; try apply Int64.unsigned_range.
+      replace (Z.of_nat (Z.to_nat i)) with i; try lia.
+      rewrite zlength_added_list; lia.
+      autorewrite with sublist.
+      rewrite zlength_added_list; lia.
+      rewrite Zlength_sublist; try lia.
+      autorewrite with sublist.
+      rewrite zlength_added_list; lia.
+      autorewrite with sublist.
+      rewrite zlength_added_list; lia.
+   
+   rewrite data_at_r.
+   cancel.
+
+
+(* Need Red. *)
+
+
+
+
+
+   
+   
+
+
+(* void curve448AddInt(uint32_t *r, const uint32_t *a, uint32_t b)
+{
+uint_t i;
+uint64_t temp;
+
+//Compute R = A + B
+temp = b; 
+for(i = 0; i < 14; i++)
+{
+   temp += a[i];
+   r[i] = temp & 0xFFFFFFFF;
+   temp >>= 32;
+}
+
+//Perform modular reduction
+curve448Red(r, r, (uint32_t) temp);
+} *)
+
+(* Loop Analysis {
+temp starts being b. Then it will either be 1 or 0.
+If temp = b and we are inside the loop then i = 0.
+   temp = b -> i = 0.
+If temp = 1 then
+   - temp + a[i] >= 2^32
+   which can only happen if:
+   - b + a[0] >= 2^32
+   - temp = 1 and a[i] = -1
+}*)
