verif_curve448Red_proofattempt.v
@@ -1,0 +1,451 @@
+Require Import VST.floyd.proofauto.
+Require Import curve448.
+Require Import list_int_functions.
+Require Import stdpp.list.
+Require Import ZArith.
+Require Import compcert.lib.Coqlib.
+Require Import list_lemmas.
+
+Instance CompSpecs : compspecs. Proof. make_compspecs prog. Defined.
+Definition Vprog : varspecs.  mk_varspecs prog. Defined.
+
+Local Open Scope Z.
+
+(* curve448Red proof attemp*)
+
+Definition prime: Z := 2^448 - 2^224 - 1.
+Definition prime_list : list Z := [-1; -1; -1; -1; -1; -1; -1;
+                                   -2; -1; -1; -1; -1; -1; -1].
+
+Definition undef14 := 
+       [Vundef; Vundef; Vundef; Vundef; Vundef; Vundef; Vundef; 
+        Vundef; Vundef; Vundef; Vundef; Vundef; Vundef; Vundef].
+
+Definition curve448Red_spec : ident * funspec :=
+DECLARE _curve448Red
+WITH    r : val,
+        shr : share,
+        a : val,
+        contents_a : list Z,
+        h : Z, (* may need writable share *)
+        gv : globals
+PRE [ tptr tuint, tptr tuint, tuint ]
+    PROP   (writable_share shr;
+            Zlength contents_a = 14;
+            0 <= (list_to_int contents_a) < (2 * prime);
+            forall x : Z, In x contents_a → x < 2 ^ 32 /\ x mod Int.modulus < 2^32
+            (*TODO  * @param[in] h The highest term of A*))
+    PARAMS (r ; a ; Vint(Int.repr h)) GLOBALS (gv)
+    SEP    (data_at_ shr (tarray tuint 14) r;
+            data_at Tsh (tarray tuint 14) (map Vint (map Int.repr contents_a)) a)
+POST [ tvoid ]
+    PROP   ()
+    RETURN ()                               
+    SEP    (data_at shr (tarray tuint 14) (* r contains the representation of A mod p *)
+   (*cont*)(map Vint (map Int.repr (int_to_list ((list_to_int contents_a) mod prime)))) r ;
+            data_at Tsh (tarray tuint 14) (map Vint (map Int.repr contents_a)) a).
+
+
+Fixpoint allprev_mone_aux (n : nat) (a : list Z) : bool :=
+   match n with 
+   | O   => true
+   | S n' => (Int.eq (Int.repr (Znth (Z.of_nat n') a)) Int.mone) 
+            && allprev_mone_aux n' a
+   end.
+   
+Definition allprev_mone (i : Z) (a : list Z) := allprev_mone_aux (Z.to_nat i) a.
+
+            
+Definition curve448Red_INV_1    (a : val)  (contents_a : list Z) 
+                     (b : val)  (r : val) (shr : share)
+                     (h : Z) (gv : globals) 
+:= 
+    (EX i : Z,
+    (PROP   (Zlength contents_a = 14)
+    LOCAL   (temp _temp (if allprev_mone i contents_a 
+               then Vlong Int64.one else Vlong Int64.zero);
+            lvar _b (tarray tuint 14) b; 
+            gvars gv; 
+            temp _a a; temp _h (Vint (Int.repr h)))
+    SEP     ( 
+                data_at_ shr (tarray tuint 14) r;
+                data_at Tsh (tarray tuint 14) (map Vint (map Int.repr contents_a)) a; 
+                data_at Tsh (tarray tuint 14)  
+                ((sublist.sublist 0 i (map Vint (map Int.repr (int_to_list ((list_to_int contents_a) - prime)))))
+                ++ sublist.sublist i 14 undef14) b
+            )))%assert.
+                
+Definition Gprog : funspecs := ltac:(with_library prog [ curve448Red_spec ]).
+
+
+Lemma L1 (i : Z) (a : list Z) : 0 <= i -> 
+   allprev_mone (i + 1) a = 
+   Int.eq (Int.repr (Znth i a)) Int.mone && allprev_mone i a.
+Proof.
+   intros.
+   unfold allprev_mone.
+   replace (i + 1) with (Z.succ i) by easy.
+   rewrite Z2Nat.inj_succ by apply H.
+   assert (i = Z.of_nat (Z.to_nat i)).
+      rewrite Z2Nat.id; auto.
+   rewrite H0 at 2.
+   induction (Z.to_nat i); auto.
+Qed.
+
+Lemma L2 :
+Int64.add Int64.one (Int64.repr (Int.modulus - 1)) = Int64.repr Int.modulus.
+Proof.
+   auto.
+   Qed.
+
+Lemma L3 (z : Z) : 
+0 <= z < Int64.modulus -> Int64.unsigned (Int64.repr z) = z.
+Proof.
+   intros.
+   rewrite Int64.unsigned_repr_eq.
+   rewrite Z.mod_small; auto.
+Qed.
+
+Lemma  L4' (z : Z): 
+Int.eq (Int.repr z) Int.mone = false -> z mod Int.modulus ≠ Int.modulus - 1.
+Proof.
+   intros.
+   apply int_eq_false_e in H.
+   unfold "≠".
+   intros.
+   replace (Int.modulus - 1) with (Int.modulus - 1 mod Int.modulus) in H0.
+   assert (Int.repr z = Int.repr (Int.modulus - 1)).
+   apply modulo_samerepr.
+   apply H0.
+   replace (Int.repr (Int.modulus - 1)) with (Int.repr (- 1)) in H1.
+   contradiction.
+   rewrite modulo_samerepr with (y:= Int.modulus - 1); reflexivity.
+   apply Zmod_small with (a := Int.modulus - 1) (n:= Int.modulus).
+   easy.
+Qed.
+
+Lemma L4 (z : Z) :
+Int.eq (Int.repr z) Int.mone = false -> z mod Int.modulus < Int.modulus - 1.
+Proof.
+   intros. 
+   apply int_eq_false_e in H.
+   unfold Int.mone in H.
+   apply Znot_ge_lt.
+   unfold not.
+   intros.
+   assert (Int.modulus ≠ 0) by easy.
+   apply Z.mod_bound_or with (a := z) in H1.
+   destruct H1.
+   destruct H1.
+   assert (z mod Int.modulus <= Int.modulus - 1).
+   apply Zlt_succ_le.
+   replace (Z.succ (Int.modulus - 1)) with (Int.modulus) by easy.
+   assumption.
+   assert ( z mod Int.modulus = Int.modulus - 1). 
+   apply Z.ge_le in H0.
+   apply Z.le_antisymm; assumption.
+   replace (Int.modulus - 1) with (- 1 mod Int.modulus) in H4 by easy.
+   apply modulo_samerepr in H4.
+   contradiction.
+   destruct H1.
+   assert (Int.modulus < 0).
+   apply Z.lt_le_trans with (m:= z mod Int.modulus); assumption.
+   discriminate H3. 
+   Qed.
+
+Lemma L5 (z : Z) : 0 <= z < two_p 32 ->
+   Int64.shru (Int64.repr z) (Int64.repr 32) = Int64.zero.
+Proof.
+   intros.
+   rewrite Int64.shru_div_two_p. 
+   assert (Int64.unsigned (Int64.repr z) / two_p (Int64.unsigned (Int64.repr 32)) = 0).
+   rewrite Zdiv_small; try easy.
+   split.
+   destruct H.
+   rewrite L3; try easy.
+   split; try easy.
+   assert ((two_p 32) < Int64.modulus) by easy.
+   apply Z.lt_trans with (two_p 32); assumption.
+   replace (Int64.unsigned (Int64.repr 32)) with 32 by easy.
+   destruct H.
+   rewrite L3; try easy.
+   split; try easy.
+   assert ((two_p 32) < Int64.modulus) by easy.
+   apply Z.lt_trans with (two_p 32); assumption.
+   rewrite H0. easy.
+   Qed. 
+
+   (*****************************)
+(* Compute Int64.unsigned (Int64.repr (2^32-1)). *)
+(* Search Int.repr (Int64.unsigned(_)). 
+Compute (Int.repr (-1)).
+Compute Int.mone.
+Compute (int_to_list (prime)).
+Compute ((prime) - 
+list_to_int([2^32+1; 4294967295; 4294967295; 4294967295; 4294967295;
+4294967295; 4294967295; 4294967295; 4294967295; 4294967295;
+4294967295; 4294967295; 4294967295; 4294967295])). *)
+
+Lemma repr_eq_32_64: forall n:Z, 
+   Int.repr (Int64.unsigned (Int64.repr (n))) = Int.repr (Int.unsigned (Int.repr (n))).
+Proof.
+   intros.
+   rewrite Int64.unsigned_repr_eq.
+   rewrite Int.unsigned_repr_eq.
+   rewrite modulo_samerepr with (y:= n mod Int.modulus); try easy.
+   replace (Int64.modulus) with (Int.modulus * Int.modulus) by easy.
+   rewrite Zaux.Zmod_mod_mult; try easy.
+   symmetry; apply Zmod_mod.    
+Qed.   
+
+Lemma L6: forall x : Z,
+0 <= x < Int.modulus -> Int64.unsigned (Int64.repr x) = Int.unsigned (Int.repr x).
+Proof.
+   intros.
+   Search (Int64.unsigned _ = Int.unsigned _).
+   assert (x = Int.unsigned(Int.repr x)).
+   rewrite Int.unsigned_repr_eq.
+   Search (_ mod _ = _).
+   rewrite Z.mod_small; try lia.
+   rewrite H0.
+   rewrite Int64.int_unsigned_repr.
+   rewrite H0 at 1.
+   easy.
+Qed.
+
+Lemma L7: 
+forall x y,
+0 <= x < Int.modulus -> 0 < y <= 32 -> 
+(Z.land x (Z.ones y)) mod Int.modulus = Z.land x (Z.ones y).
+Proof.
+   intros.
+   rewrite Z.mod_small; try easy.
+   split.
+   apply Z.land_nonneg.
+   lia. 
+   rewrite Z.land_ones; try lia.
+   replace (Int.modulus) with (2^32) by easy.
+   assert (A1 : x mod 2 ^ y < 2^y).
+   apply Z.mod_pos_bound; lia.
+   assert (A2 : 2 ^ y <= 2 ^ 32).
+   destruct H0.
+   apply Z.pow_le_mono_r; try lia.
+   apply Z.lt_le_trans with (m:= 2^y); try lia.
+Qed.
+
+   (*****************************)
+
+Lemma body_curve448Red : semax_body Vprog Gprog f_curve448Red curve448Red_spec.
+Proof.
+   start_function.
+   forward.
+   forward_for_simple_bound 7 
+      (curve448Red_INV_1 a contents_a v_b r shr h gv).
+   entailer!.
+   apply derives_refl.
+   repeat forward.
+   entailer!.
+   rewrite L1 by easy.
+   destruct (allprev_mone i contents_a) eqn:E1;
+   destruct (Int.eq (Int.repr (Znth i contents_a)) Int.mone) eqn:E2;
+   simpl; f_equal; remember (Znth i contents_a) as x.
+     apply Int.same_if_eq in E2.
+      rewrite E2, Int.unsigned_mone.
+      easy.
+     unfold Int64.add.
+      assert (A : 0 <= x mod Int.modulus < Int64.modulus).
+         assert (A0 : 0 < Int.modulus) by easy.
+         pose proof (Z.mod_pos_bound x Int.modulus A0); clear A0.
+         assert (A0 : Int.modulus < Int64.modulus) by easy.
+         destruct H10.
+         discriminate H9.
+         destruct H11.
+         pose proof (Z.lt_trans (x mod Int.modulus) Int.modulus Int64.modulus H13 A0);
+         split; try easy.
+      rewrite Int64.unsigned_one, L5; try rewrite !Int.unsigned_repr_eq;
+         try rewrite L3; try easy. 
+      split.
+      assert (A0 : 0 < Int.modulus) by easy.
+      pose proof (Z.mod_pos_bound x Int.modulus A0); clear A0.
+      rewrite (Z.add_nonneg_nonneg 1 (x mod Int.modulus)); easy.
+      replace (32 mod Int.modulus) with (32) by easy.
+      apply L4 in E2.
+      apply Zplus_lt_compat_l with (p := 1) in E2.
+      replace (1 + (Int.modulus - 1)) with Int.modulus in E2 by lia.
+      replace (two_p 32) with (Int.modulus) by easy; auto.
+     apply Int.same_if_eq in E2.
+      rewrite E2, Int.unsigned_mone.
+      easy.
+     rewrite Int64.add_zero_l, !Int.unsigned_repr_eq.
+      replace (32 mod Int.modulus) with (32) by easy.
+      rewrite L5; auto.
+      replace (two_p 32) with (Int.modulus) by easy.
+      assert (A0 : 0 < Int.modulus) by easy.
+      pose proof (Z.mod_pos_bound x Int.modulus A0); clear A0.
+      apply H11.
+      (* Prove that if loop inv holds after i then it holds after doing the 
+         i+1 iteration. *)
+      destruct  (allprev_mone i contents_a) eqn:E.
+         (* Case allprev_mone i contents_a = true. Means temp = 1. *)      
+         assert ((upd_Znth i
+            (sublist.sublist 0 i
+               (map Vint
+                  (map Int.repr (int_to_list (list_to_int contents_a - prime)))) ++
+            sublist.sublist i 14 undef14)
+            (force_val
+               (sem_cast_l2i I32 Unsigned
+                  (force_val
+                     (sem_and tulong tuint
+                        (force_val
+                           (both_long
+                              (λ n1 n2 : int64, Some (Vlong (Int64.add n1 n2)))
+                              sem_cast_pointer (sem_cast_i2l Unsigned)
+                              (Vlong Int64.one)
+                              (Vint (Int.repr (Znth i contents_a)))))
+                        (Vint (Int.repr (-1)))))))) 
+      = (sublist.sublist 0 (i + 1)
+               (map Vint
+                  (map Int.repr (int_to_list (list_to_int contents_a - prime)))) ++
+            sublist.sublist (i + 1) 14 undef14) 
+         ) as H_v_b.
+
+      rewrite <- !(sublist_rejoin 0 i (i+1)); try easy.
+      rewrite <- app_assoc.   
+      rewrite upd_list_app_upper.
+      rewrite Zlength_sublist; try easy.
+      autorewrite with sublist.  
+      rewrite sublist_update_0th_gen; try easy; try lia.
+      repeat f_equal.
+
+      rewrite sublist_len_1.
+      rewrite Znth_map_Vint_map_Int_repr.
+      simpl.   (* simpl works really well here! *)
+      f_equal; f_equal. 
+      unfold Int64.and.
+      rewrite repr_eq_32_64.
+      unfold Int64.add.
+      rewrite Int64.unsigned_one.
+      rewrite Int.unsigned_repr_eq.
+      (* rewrite modulo_samerepr with ( y:= (Znth i (int_to_list (list_to_int contents_a - prime)))); try easy. *)
+      replace (Int64.unsigned (Int64.repr (Int.unsigned (Int.repr (-1))))) with (Z.ones 32) by easy.
+      rewrite Int.unsigned_repr_eq.
+      (* replace (i) with (Z.of_nat (Z.to_nat i)) by lia.
+      rewrite Znth_int_to_list.
+      replace (Z.of_nat (Z.to_nat i)) with i by lia. *)
+      rewrite L6. 
+      rewrite L6.
+      replace (Int.unsigned (Int.repr (Znth i contents_a mod Int.modulus)))
+         with (Znth i contents_a mod Int.modulus).
+      rewrite L7; try easy; try apply Int.unsigned_range.
+      rewrite Z.land_ones; try easy.
+      rewrite Int.unsigned_repr_eq.
+      replace (Int.modulus) with (2^32) by easy.
+      repeat rewrite Z.mod_mod; try easy.   
+      replace (2 ^ (32 * i)) with 
+         (two_p (Int.unsigned(Int.repr ((32 * i))))).
+      replace ((list_to_int contents_a - prime)) with (Int.unsigned (Int.repr ((list_to_int contents_a - prime)))).
+      replace (Int.repr
+      ((Int.unsigned (Int.repr (list_to_int contents_a - prime)) /
+        two_p (Int.unsigned (Int.repr (32 * i)))))) with Int.zero. (*BAD*)
+        rewrite <- Int.shru_div_two_p.
+
+
+
+
+      apply modulo_samerepr.
+      (* shru_div_two_p
+      Search Int.shru.
+      two_p_equiv
+          *)
+      apply H1.
+      
+
+      (* HERE *)
+      assert ((Znth i contents_a = -1) \/ (Znth i contents_a <> -1)) by
+      lia.
+      destruct H10; try rewrite H10.
+      replace ((Int64.add Int64.one (Int64.repr (Int.unsigned (Int.repr (-1)))))) 
+         with (Int64.repr(2^32)) by easy.
+      replace ((Int64.and (Int64.repr (2 ^ 32))
+      (Int64.repr (Int.unsigned (Int.repr (-1)))))) with (Int64.zero) by easy.
+      replace (Int.repr (Int64.unsigned Int64.zero)) with (Int.repr 0) by easy.
+
+
+      assert (((list_to_int contents_a - prime) / 2 ^ (32 * i)) mod 2 ^ 32= 
+         ((list_to_int contents_a) / 2 ^ (32 * i)) mod 2 ^ 32
+            -((prime) / 2 ^ (32 * i)) mod 2 ^ 32).
+
+      simpl.
+      Search (_ - _ mod _).
+      
+      rewrite eq_dec.
+      assert (Int64.and
+      (Int64.add Int64.one
+         (Int64.repr (Int.unsigned (Int.repr (Znth i contents_a)))))
+      (Int64.repr (Int.unsigned (Int.repr (-1)))) = 
+      Int64.repr( Int64.intval (Int64.and
+            (Int64.add Int64.one 
+               (Int64.repr (Int.unsigned (Int.repr (Znth i contents_a)))))
+            (Int64.repr (Int.unsigned (Int.repr (-1))))))).
+      
+      unfold Int64.and.
+      
+      
+
+      (*****************************)
+
+      admit.
+         
+      autorewrite with sublist; rewrite int_to_list_length; lia.
+      autorewrite with sublist; rewrite int_to_list_length; lia.
+      
+      rewrite Zlength_sublist; try lia.
+      autorewrite with sublist; rewrite int_to_list_length; lia.
+      autorewrite with sublist; rewrite int_to_list_length; lia.
+
+      rewrite H_v_b; cancel.
+      
+      assert(upd_Znth i
+      (sublist.sublist 0 i (map Vint (map Int.repr (int_to_list (list_to_int contents_a mod prime)))) ++
+         sublist.sublist i 14 undef14)
+      (force_val
+         (sem_cast_l2i I32 Unsigned
+            (force_val
+               (sem_and tulong tuint
+                  (force_val
+                     (both_long (λ n1 n2 : int64, Some (Vlong (Int64.add n1 n2))) sem_cast_pointer
+                        (sem_cast_i2l Unsigned) (Vlong Int64.zero) (Vint (Int.repr (Znth i contents_a)))))
+                  (Vint (Int.repr (-1))))))) 
+         = sublist.sublist 0 (i + 1) (map Vint (map Int.repr (int_to_list (list_to_int contents_a mod prime)))) ++
+         sublist.sublist (i + 1) 14 undef14).
+         
+      rewrite <- !(sublist_rejoin 0 i (i+1)); try easy.
+      rewrite <- app_assoc.   
+      rewrite upd_list_app_upper.
+      rewrite Zlength_sublist; try easy.
+      autorewrite with sublist.  
+      rewrite sublist_update_0th_gen; try easy; try lia.
+      rewrite sublist_len_1.
+      repeat f_equal.
+      simpl.
+
+      Compute (Int64.repr (Int.unsigned (Int.repr (-1)))).
+      Compute (Int64.repr (2^32-1)).
+         (*****************************)
+
+      (* Need to show that (int_to_list list_to_int) combo preserves length. *)
+
+
+   (* I proved (modulo the lemmas L1--L5) the part that the contents of
+   * temp is as defined in the loop invariant.
+   * The part that the contents of b are as in the loop invariant is ugly. 
+   * One need to prove that whatever its been done
+   * in the code with the temp is does indeed the least significant 7 limbs
+   * of B = A - (2^448 - 2^224 - 1). A Lemma (or several) are needed.
+   *)
+
+
+
+      
+      
+      
